Fix compilation in all proofs.

language_formalisation/type_system/type_aux_lemmas.v
@@ -11,13 +11,6 @@ Require Export subs_lemmas wellfounded_lemmas.
 Ltac inv H := inversion H; clear H; subst.
 
 
-Lemma extend_get_proof Γ A i Ai:
-  get_vtype Γ i = Some Ai-> get_vtype (CtxU Γ A) (i + 1) = Some Ai.
-Proof.
-assert (i + 1 = S i) by omega.
-induction Γ; rewrite H; auto.
-Qed.
-
 Fixpoint v_insert_typesafe v Γ A A_ins i {struct v} :
   has_vtype Γ v A -> wf_vtype A_ins ->
   has_vtype (ctx_insert_var Γ A_ins i) (Sub.v_shift v 1 i) A
@@ -152,584 +145,315 @@ inv orig. destruct h.
 Qed.
 
 
-
-Proof.
-{
-clear v_insert_typesafe.
-revert A i. induction v.
-+ clear c_insert_typesafe h_insert_typesafe.
-  intros. inv H. inv H3. simpl.
-  apply TypeV. apply ctx_insert_wf; assumption. assumption.
-  assert (
-    (if i <=? num then (name, num + 1) else (name, num))
-      = (name, if i <=? num then num + 1 else num) ) 
-  as same by (destruct (i<=?num); reflexivity).
-  rewrite same. simpl. apply TypeVar.
-  simpl. destruct (i<=?num) eqn:cmp.
-  - erewrite <-get_ctx_insert_changed.
-    * assumption.
-    * apply leb_complete in cmp. omega.
-  - erewrite <-get_ctx_insert_unchanged.
-    * assumption.
-    * apply leb_iff_conv in cmp. omega.
-+ clear c_insert_typesafe h_insert_typesafe.
-  intros. inv H. inv H3. simpl.
-  apply TypeV. apply ctx_insert_wf; assumption. assumption. apply TypeUnit.
-+ clear c_insert_typesafe h_insert_typesafe.
-  intros. inv H. inv H3. simpl.
-  apply TypeV. apply ctx_insert_wf; assumption. assumption. apply TypeInt.
-+ clear c_insert_typesafe h_insert_typesafe.
-  intros. inv H. inv H3. simpl.
-  apply TypeV. apply ctx_insert_wf; assumption. assumption.
-  apply TypeInl. apply IHv; assumption.
-+ clear c_insert_typesafe h_insert_typesafe.
-  intros. inv H. inv H3. simpl.
-  apply TypeV. apply ctx_insert_wf; assumption. assumption.
-  apply TypeInr. apply IHv; assumption.
-+ clear c_insert_typesafe h_insert_typesafe.
-  intros. inv H. inv H3. simpl.
-  apply TypeV. apply ctx_insert_wf; assumption. assumption.
-  apply TypePair. apply IHv1; assumption. apply IHv2; assumption.
-+ clear h_insert_typesafe.
-  intros. inv H. inv H3.
-  apply TypeV. apply ctx_insert_wf; assumption. assumption.
-  simpl. apply TypeFun. rewrite ctx_insert_extend.
-  apply c_insert_typesafe; assumption.
-+ intros. inv H. inv H3. simpl.
-  apply TypeV. apply ctx_insert_wf; assumption. assumption.
-  simpl. apply TypeHandler. rewrite ctx_insert_extend. apply c_insert_typesafe.
-  clear c_insert_typesafe.
-  assumption. assumption.
-  apply h_insert_typesafe. assumption. assumption.
-}{
-clear c_insert_typesafe h_insert_typesafe.
-revert Γ C i. induction c.
-+ intros. inv H. inv H3.
-  apply TypeC. apply ctx_insert_wf; assumption. assumption.
-  simpl. apply TypeRet. apply v_insert_typesafe; assumption.
-+ intros. inv H. inv H3.
-  apply TypeC. apply ctx_insert_wf; assumption. assumption.
-  simpl. eapply TypeΠMatch.
-  - apply v_insert_typesafe. exact H8. assumption.
-  - clear v_insert_typesafe. 
-    rewrite ctx_insert_extend. rewrite ctx_insert_extend.
-    assert (i+1+1=i+2) by omega. rewrite H. apply IHc; assumption.
-+ intros. inv H. inv H3.
-  apply TypeC. apply ctx_insert_wf; assumption. assumption.
-  simpl. eapply TypeΣMatch.
-  - clear IHc1 IHc2. apply v_insert_typesafe. exact H10. assumption.
-  - clear v_insert_typesafe IHc2. rewrite ctx_insert_extend. apply IHc1; assumption.
-  - clear v_insert_typesafe IHc1. rewrite ctx_insert_extend. apply IHc2; assumption.
-+ intros. inv H. inv H3.
-  apply TypeC. apply ctx_insert_wf; assumption. assumption.
-  simpl. eapply TypeApp.
-  - apply v_insert_typesafe. exact H6. assumption.
-  - apply v_insert_typesafe; assumption.
-+ intros. inv H. inv H3.
-  apply TypeC. apply ctx_insert_wf; assumption. assumption.
-  simpl. eapply TypeOp.
-  - exact H9.
-  - clear IHc. apply v_insert_typesafe; assumption.
-  - clear v_insert_typesafe. rewrite ctx_insert_extend. apply IHc; assumption.
-+ clear v_insert_typesafe. intros. inv H. inv H3.
-  apply TypeC. apply ctx_insert_wf; assumption. assumption.
-  simpl. eapply TypeLetRec.
-  - clear IHc2. rewrite ctx_insert_extend. rewrite ctx_insert_extend.
-    assert (i+1+1=i+2) by omega. rewrite H. apply IHc1. exact H9. assumption.
-  - clear IHc1. rewrite ctx_insert_extend. apply IHc2; assumption.
-+ clear v_insert_typesafe. intros. inv H. inv H3.
-  apply TypeC. apply ctx_insert_wf; assumption. assumption.
-  simpl. eapply TypeDoBind.
-  - clear IHc2. apply IHc1. exact H8. assumption.
-  - clear IHc1. rewrite ctx_insert_extend. apply IHc2; assumption.
-+ intros. inv H. inv H3.
-  apply TypeC. apply ctx_insert_wf; assumption. assumption.
-  simpl. eapply TypeHandle.
-  - clear IHc. apply v_insert_typesafe. exact H6. assumption.
-  - clear v_insert_typesafe. apply IHc; assumption.
-}{
-clear h_insert_typesafe v_insert_typesafe.
-revert Γ Σ D i. induction h; intros Γ Σ D i orig wf_Ains; simpl; 
-inv orig; inv H0; inv H1; apply TypeH; try (apply ctx_insert_wf; assumption); 
-try apply WfSigØ || apply WfCty || apply WfSigU; try assumption.
-+ clear c_insert_typesafe. apply TypeCasesØ.
-+ clear c_insert_typesafe. inv H2.
-+ clear c_insert_typesafe. inv H2.
-+ inv H2. apply TypeCasesU.
-  - clear c_insert_typesafe IHh. 
-    assert (forall h,
-      find_op_case h op = None ->
-      find_op_case (Sub.h_shift h 1 i) op = None).
-    * intros h' orig. induction h'. assumption.
-      simpl in *. destruct (op==o). discriminate. apply IHh'; assumption.
-    * apply H1. assumption.
-  - clear c_insert_typesafe. apply IHh; assumption.
-  - clear IHh. rewrite ctx_insert_extend. rewrite ctx_insert_extend.
-    assert (i+1+1=i+2) by omega. rewrite H1.
-    apply c_insert_typesafe; assumption.
-}
-Qed.
-
-Fixpoint v_insert_typesafe Γ v A A_ins i {struct v} :
-  has_vtype Γ v A -> wf_vtype A_ins ->
-  has_vtype (ctx_insert_var Γ A_ins i) (Sub.v_shift v 1 i) A
-with c_insert_typesafe Γ c C A_ins i {struct c} :
-  has_ctype Γ c C -> wf_vtype A_ins ->
-  has_ctype (ctx_insert_var Γ A_ins i) (Sub.c_shift c 1 i) C
-with h_insert_typesafe Γ h Σ D A_ins i {struct h} :
-  has_htype Γ h Σ D -> wf_vtype A_ins ->
-  has_htype (ctx_insert_var Γ A_ins i) (Sub.h_shift h 1 i) Σ D.
-Proof.
-{
-clear v_insert_typesafe.
-revert A i. induction v.
-+ clear c_insert_typesafe h_insert_typesafe.
-  intros. inv H. inv H3. simpl.
-  apply TypeV. apply ctx_insert_wf; assumption. assumption.
-  assert (
-    (if i <=? num then (name, num + 1) else (name, num))
-      = (name, if i <=? num then num + 1 else num) ) 
-  as same by (destruct (i<=?num); reflexivity).
-  rewrite same. simpl. apply TypeVar.
-  simpl. destruct (i<=?num) eqn:cmp.
-  - erewrite <-get_ctx_insert_changed.
-    * assumption.
-    * apply leb_complete in cmp. omega.
-  - erewrite <-get_ctx_insert_unchanged.
-    * assumption.
-    * apply leb_iff_conv in cmp. omega.
-+ clear c_insert_typesafe h_insert_typesafe.
-  intros. inv H. inv H3. simpl.
-  apply TypeV. apply ctx_insert_wf; assumption. assumption. apply TypeUnit.
-+ clear c_insert_typesafe h_insert_typesafe.
-  intros. inv H. inv H3. simpl.
-  apply TypeV. apply ctx_insert_wf; assumption. assumption. apply TypeInt.
-+ clear c_insert_typesafe h_insert_typesafe.
-  intros. inv H. inv H3. simpl.
-  apply TypeV. apply ctx_insert_wf; assumption. assumption.
-  apply TypeInl. apply IHv; assumption.
-+ clear c_insert_typesafe h_insert_typesafe.
-  intros. inv H. inv H3. simpl.
-  apply TypeV. apply ctx_insert_wf; assumption. assumption.
-  apply TypeInr. apply IHv; assumption.
-+ clear c_insert_typesafe h_insert_typesafe.
-  intros. inv H. inv H3. simpl.
-  apply TypeV. apply ctx_insert_wf; assumption. assumption.
-  apply TypePair. apply IHv1; assumption. apply IHv2; assumption.
-+ clear h_insert_typesafe.
-  intros. inv H. inv H3.
-  apply TypeV. apply ctx_insert_wf; assumption. assumption.
-  simpl. apply TypeFun. rewrite ctx_insert_extend.
-  apply c_insert_typesafe; assumption.
-+ intros. inv H. inv H3. simpl.
-  apply TypeV. apply ctx_insert_wf; assumption. assumption.
-  simpl. apply TypeHandler. rewrite ctx_insert_extend. apply c_insert_typesafe.
-  clear c_insert_typesafe.
-  assumption. assumption.
-  apply h_insert_typesafe. assumption. assumption.
-}{
-clear c_insert_typesafe h_insert_typesafe.
-revert Γ C i. induction c.
-+ intros. inv H. inv H3.
-  apply TypeC. apply ctx_insert_wf; assumption. assumption.
-  simpl. apply TypeRet. apply v_insert_typesafe; assumption.
-+ intros. inv H. inv H3.
-  apply TypeC. apply ctx_insert_wf; assumption. assumption.
-  simpl. eapply TypeΠMatch.
-  - apply v_insert_typesafe. exact H8. assumption.
-  - clear v_insert_typesafe. 
-    rewrite ctx_insert_extend. rewrite ctx_insert_extend.
-    assert (i+1+1=i+2) by omega. rewrite H. apply IHc; assumption.
-+ intros. inv H. inv H3.
-  apply TypeC. apply ctx_insert_wf; assumption. assumption.
-  simpl. eapply TypeΣMatch.
-  - clear IHc1 IHc2. apply v_insert_typesafe. exact H10. assumption.
-  - clear v_insert_typesafe IHc2. rewrite ctx_insert_extend. apply IHc1; assumption.
-  - clear v_insert_typesafe IHc1. rewrite ctx_insert_extend. apply IHc2; assumption.
-+ intros. inv H. inv H3.
-  apply TypeC. apply ctx_insert_wf; assumption. assumption.
-  simpl. eapply TypeApp.
-  - apply v_insert_typesafe. exact H6. assumption.
-  - apply v_insert_typesafe; assumption.
-+ intros. inv H. inv H3.
-  apply TypeC. apply ctx_insert_wf; assumption. assumption.
-  simpl. eapply TypeOp.
-  - exact H9.
-  - clear IHc. apply v_insert_typesafe; assumption.
-  - clear v_insert_typesafe. rewrite ctx_insert_extend. apply IHc; assumption.
-+ clear v_insert_typesafe. intros. inv H. inv H3.
-  apply TypeC. apply ctx_insert_wf; assumption. assumption.
-  simpl. eapply TypeLetRec.
-  - clear IHc2. rewrite ctx_insert_extend. rewrite ctx_insert_extend.
-    assert (i+1+1=i+2) by omega. rewrite H. apply IHc1. exact H9. assumption.
-  - clear IHc1. rewrite ctx_insert_extend. apply IHc2; assumption.
-+ clear v_insert_typesafe. intros. inv H. inv H3.
-  apply TypeC. apply ctx_insert_wf; assumption. assumption.
-  simpl. eapply TypeDoBind.
-  - clear IHc2. apply IHc1. exact H8. assumption.
-  - clear IHc1. rewrite ctx_insert_extend. apply IHc2; assumption.
-+ intros. inv H. inv H3.
-  apply TypeC. apply ctx_insert_wf; assumption. assumption.
-  simpl. eapply TypeHandle.
-  - clear IHc. apply v_insert_typesafe. exact H6. assumption.
-  - clear v_insert_typesafe. apply IHc; assumption.
-}{
-clear h_insert_typesafe v_insert_typesafe.
-revert Γ Σ D i. induction h; intros Γ Σ D i orig wf_Ains; simpl; 
-inv orig; inv H0; inv H1; apply TypeH; try (apply ctx_insert_wf; assumption); 
-try apply WfSigØ || apply WfCty || apply WfSigU; try assumption.
-+ clear c_insert_typesafe. apply TypeCasesØ.
-+ clear c_insert_typesafe. inv H2.
-+ clear c_insert_typesafe. inv H2.
-+ inv H2. apply TypeCasesU.
-  - clear c_insert_typesafe IHh. 
-    assert (forall h,
-      find_op_case h op = None ->
-      find_op_case (Sub.h_shift h 1 i) op = None).
-    * intros h' orig. induction h'. assumption.
-      simpl in *. destruct (op==o). discriminate. apply IHh'; assumption.
-    * apply H1. assumption.
-  - clear c_insert_typesafe. apply IHh; assumption.
-  - clear IHh. rewrite ctx_insert_extend. rewrite ctx_insert_extend.
-    assert (i+1+1=i+2) by omega. rewrite H1.
-    apply c_insert_typesafe; assumption.
-}
-Qed.
-
-(*
-Fixpoint v_insert_typesafe Γ v A A_ins i {struct v} :
-  has_vtype Γ v A -> wf_vtype A_ins ->
-  has_vtype (ctx_insert_var Γ A_ins i) (Sub.v_shift v 1 i) A
-with c_insert_typesafe Γ c C A_ins i {struct c} :
-  has_ctype Γ c C -> wf_vtype A_ins ->
-  has_ctype (ctx_insert_var Γ A_ins i) (Sub.c_shift c 1 i) C
-with h_insert_typesafe Γ h Σ D A_ins i {struct h} :
-  has_htype Γ h Σ D -> wf_vtype A_ins ->
-  has_htype (ctx_insert_var Γ A_ins i) (Sub.h_shift h 1 i) Σ D.
-Proof.
-{
-clear v_insert_typesafe.
-revert A i. induction v; intros A i orig wf_Ains.
-Focus 7. 
-  clear h_insert_typesafe. inv orig. inv H1. apply TypeV.
-  apply ctx_insert_wf. assumption. assumption.
-  assumption.
-  simpl. apply TypeFun. rewrite ctx_insert_extend. apply c_insert_typesafe.
-  assumption. assumption.
-Focus 7.
-  inv orig. inv H1. apply TypeV.
-  apply ctx_insert_wf. assumption. assumption.
-  assumption.
-  simpl. apply TypeHandler. rewrite ctx_insert_extend. apply c_insert_typesafe.
-  assumption. assumption.
-  apply h_insert_typesafe. assumption. assumption.
- 
-all: clear c_insert_typesafe h_insert_typesafe.
-all: inv orig; inv H1; apply TypeV; try (assumption || apply ctx_insert_wf; assumption).
-+ simpl. assert (
-    (if i <=? num then (name, num + 1) else (name, num))
-      = (name, if i <=? num then num + 1 else num) ) 
-  as same by (destruct (i<=?num); reflexivity).
-  rewrite same. apply TypeVar. simpl. 
-  simpl. destruct (i<=?num) eqn:cmp.
-  - erewrite <-get_ctx_insert_changed.
-    * assumption.
-    * apply leb_complete in cmp. omega.
-  - erewrite <-get_ctx_insert_unchanged.
-    * assumption.
-    * apply leb_iff_conv in cmp. omega.
-+ apply TypeUnit.
-+ apply TypeInt.
-+ apply TypeInl. apply IHv; assumption.
-+ apply TypeInr. apply IHv; assumption.
-+ apply TypePair; try apply IHv1 || apply IHv2; assumption.
-}{
-clear c_insert_typesafe h_insert_typesafe.
-revert Γ C i. induction c; intros Γ C i orig wfAins; simpl;
-inv orig; inv H1; apply TypeC; try (assumption || apply ctx_insert_wf; assumption).
-+ apply TypeRet. apply v_insert_typesafe; assumption.
-+ eapply TypeΠMatch.
-  - eapply v_insert_typesafe. exact H7. assumption.
-  - rewrite ctx_insert_extend. rewrite ctx_insert_extend.
-    assert (i+1+1=i+2) by omega. rewrite H1. apply IHc; assumption.
-+ eapply TypeΣMatch.
-  - apply v_insert_typesafe. exact H9. assumption.
-  - rewrite ctx_insert_extend. apply IHc1; assumption.
-  - rewrite ctx_insert_extend. apply IHc2; assumption.
-+ eapply TypeApp.
-  - apply v_insert_typesafe. exact H5. assumption.
-  - apply v_insert_typesafe; assumption.
-+ eapply TypeOp. exact H8. 
-  - apply v_insert_typesafe; assumption.
-  - rewrite ctx_insert_extend. apply IHc; assumption.
-+ eapply TypeLetRec.
-  - rewrite ctx_insert_extend. rewrite ctx_insert_extend.
-    assert (i+1+1=i+2) by omega. rewrite H1. apply IHc1. exact H8. assumption.
-  - rewrite ctx_insert_extend. apply IHc2; assumption.
-+ eapply TypeDoBind.
-  - apply IHc1. exact H7. assumption.
-  - rewrite ctx_insert_extend. apply IHc2; assumption.
-+ eapply TypeHandle.
-  - apply v_insert_typesafe. exact H5. assumption.
-  -  apply IHc; assumption.
-}{
-clear h_insert_typesafe v_insert_typesafe.
-revert Γ Σ D i. induction h; intros Γ Σ D i orig wf_Ains; simpl; 
-inv orig; inv H0; inv H1; apply TypeH; try (apply ctx_insert_wf; assumption); 
-try apply WfSigØ || apply WfCty || apply WfSigU; try assumption.
-+ apply TypeCasesØ.
-+ inv H2.
-+ inv H2.
-+ inv H2. apply TypeCasesU; auto.
-  - assert (forall h,
-      find_op_case h op = None ->
-      find_op_case (Sub.h_shift h 1 i) op = None).
-    * intros h' orig. induction h'. assumption.
-      simpl in *. destruct (op==o). discriminate. apply IHh'; assumption.
-    * apply H1. assumption.
-  - rewrite ctx_insert_extend. rewrite ctx_insert_extend.
-    assert (i+1+1=i+2) by omega. rewrite H1.
-    apply c_insert_typesafe; assumption.
-}
-Qed.
-
-
-
-Fixpoint v_shift_typesafe
-  (Γ:ctx) (A0:vtype) v A {struct v} :
+Fixpoint v_shift_typesafe v (Γ:ctx) A0 A {struct v} :
   has_vtype Γ v A -> wf_vtype A0 ->
   has_vtype (CtxU Γ A0) (Sub.v_shift v 1 0) A
 
-with c_shift_typesafe
-  (Γ:ctx) (A0:vtype) c C {struct c} :
+with c_shift_typesafe c (Γ:ctx) A0 C {struct c} :
   has_ctype Γ c C -> wf_vtype A0 ->
   has_ctype (CtxU Γ A0) (Sub.c_shift c 1 0) C
 
-with h_shift_typesafe
-  (Γ:ctx) (A0:vtype) h Σ D {struct h} :
+with h_shift_typesafe h (Γ:ctx) A0 Σ D {struct h} :
   has_htype Γ h Σ D -> wf_vtype A0 ->
   has_htype (CtxU Γ A0) (Sub.h_shift h 1 0) Σ D.
+
 Proof.
 all: intro orig;
 assert (ctx_insert_var Γ A0 0 = CtxU Γ A0) by (destruct Γ; auto);
-rewrite <-H; inv orig.
-apply v_insert_typesafe. apply TypeV; assumption.
-apply c_insert_typesafe. apply TypeC; assumption.
-apply h_insert_typesafe. apply TypeH; assumption.
+rewrite <-H.
+apply v_insert_typesafe. assumption.
+apply c_insert_typesafe. assumption.
+apply h_insert_typesafe. assumption.
 Qed.
 
 
-Fixpoint v_negshift_typesafe
-  (Γ:ctx) v A i {struct v} :
-  has_vtype Γ v A ->
-  v_no_var_j v i ->
+Fixpoint v_negshift_typesafe v (Γ:ctx) A i {struct v} :
+  has_vtype Γ v A -> v_no_var_j v i ->
   has_vtype (ctx_remove_var Γ i) (Sub.v_negshift v 1 i) A
 
-with c_negshift_typesafe
-  (Γ:ctx) c C i {struct c} :
-  has_ctype Γ c C ->
-  c_no_var_j c i ->
+with c_negshift_typesafe c (Γ:ctx) C i {struct c} :
+  has_ctype Γ c C -> c_no_var_j c i ->
   has_ctype (ctx_remove_var Γ i) (Sub.c_negshift c 1 i) C
 
-with h_negshift_typesafe
-  (Γ:ctx) h Σ D i {struct h} :
-  has_htype Γ h Σ D ->
-  h_no_var_j h i ->
+with h_negshift_typesafe h (Γ:ctx) Σ D i {struct h} :
+  has_htype Γ h Σ D -> h_no_var_j h i ->
   has_htype (ctx_remove_var Γ i) (Sub.h_negshift h 1 i) Σ D.
 Proof.
 {
-clear v_negshift_typesafe.
-revert Γ A i. induction v; intros Γ A i orig no_var; simpl; 
-inv orig; inv H1; apply TypeV; simpl in no_var; 
-try (apply ctx_remove_wf; assumption); try assumption.
-+ simpl. assert (
+intros orig no_var. simpl in no_var. apply TypeV; inv orig.
+{ apply ctx_remove_wf. assumption. }
+{ assumption. }
+destruct v.
++ clear v_negshift_typesafe c_negshift_typesafe h_negshift_typesafe.
+  simpl. destruct v as (name, num). simpl. inv H1.
+  assert (
     (if i <=? num then (name, num - 1) else (name, num))
       = (name, if i <=? num then num - 1 else num) ) 
-  as same by (destruct (i<=?num); reflexivity).
-  rewrite same. apply TypeVar. destruct (i<=?num) eqn:cmp.
-  - erewrite <-get_ctx_remove_changed; apply leb_complete in cmp.
+    as same by (destruct (i<=?num); reflexivity).
+  rewrite same. destruct (i <=? num) eqn:cmp.
+  - apply TypeVar. rewrite <-get_ctx_remove_changed; apply leb_complete in cmp.
     * destruct num. destruct no_var. omega.
       simpl. assert (num-0=num) by omega. rewrite H1. assumption.
-    * omega.
-  - erewrite <-get_ctx_remove_unchanged. assumption.
-    apply leb_iff_conv in cmp. omega.
-+ apply TypeUnit.
-+ apply TypeInt.
-+ apply TypeInl. eapply IHv. exact H4. assumption.
-+ apply TypeInr. eapply IHv. exact H4. assumption.
-+ apply TypePair; destruct no_var.
-  - eapply IHv1. exact H5. assumption.
-  - eapply IHv2. exact H7. assumption.
-+ apply TypeFun. rewrite ctx_remove_extend.
-  apply c_negshift_typesafe; assumption.
-+ apply TypeHandler; destruct no_var.
-  - rewrite ctx_remove_extend. apply c_negshift_typesafe; assumption.
-  - apply h_negshift_typesafe; assumption.
+    * destruct cmp.
+      ++ destruct no_var. reflexivity.
+      ++ omega.
+  - apply TypeVar. rewrite <-get_ctx_remove_unchanged.
+    assumption. apply leb_iff_conv in cmp. assumption.
++ clear v_negshift_typesafe c_negshift_typesafe h_negshift_typesafe.
+  simpl. inv H1. apply TypeUnit.
++ clear v_negshift_typesafe c_negshift_typesafe h_negshift_typesafe.
+  simpl. inv H1. apply TypeInt.
++ specialize (v_negshift_typesafe v) as IHv.
+  clear v_negshift_typesafe c_negshift_typesafe h_negshift_typesafe.
+  simpl. inv H1. apply TypeInl. apply IHv.
+  assumption. assumption.
++ specialize (v_negshift_typesafe v) as IHv.
+  clear v_negshift_typesafe c_negshift_typesafe h_negshift_typesafe.
+  simpl. inv H1. apply TypeInr. apply IHv.
+  assumption. assumption.
++ specialize (v_negshift_typesafe v1) as IHv1.
+  specialize (v_negshift_typesafe v2) as IHv2.
+  clear v_negshift_typesafe c_negshift_typesafe h_negshift_typesafe.
+  simpl. inv H1. destruct no_var. apply TypePair. 
+  apply IHv1; assumption. apply IHv2; assumption.
++ specialize (c_negshift_typesafe c) as IHc.
+  clear v_negshift_typesafe c_negshift_typesafe h_negshift_typesafe.
+  simpl. inv H1. apply TypeFun. rewrite ctx_remove_extend.
+  apply IHc; assumption.
++ specialize (h_negshift_typesafe h) as IHh.
+  specialize (c_negshift_typesafe c) as IHc.
+  clear v_negshift_typesafe c_negshift_typesafe h_negshift_typesafe.
+  simpl. inv H1. destruct no_var.
+  apply TypeHandler. rewrite ctx_remove_extend.
+  apply IHc; assumption. apply IHh; assumption.
 }{
-clear c_negshift_typesafe.
-revert Γ C i. induction c; intros Γ C i orig no_var; inv orig; inv H1; inv H0;
-simpl in no_var; try destruct no_var; apply TypeC; simpl; 
-try (apply ctx_remove_wf; assumption); try (apply WfCty; assumption).
-+ apply TypeRet. apply v_negshift_typesafe; assumption.
-+ eapply TypeΠMatch.
-  - apply v_negshift_typesafe. exact H7. assumption.
+intros orig no_var. simpl in no_var. apply TypeC; inv orig.
+{ apply ctx_remove_wf. assumption. }
+{ assumption. }
+destruct c.
++ specialize (v_negshift_typesafe v) as IHv.
+  clear v_negshift_typesafe c_negshift_typesafe h_negshift_typesafe.
+  simpl. inv H1. apply TypeRet. apply IHv; assumption.
++ specialize (v_negshift_typesafe v) as IHv.
+  specialize (c_negshift_typesafe c) as IHc.
+  clear v_negshift_typesafe c_negshift_typesafe h_negshift_typesafe.
+  simpl. inv H1. destruct no_var. eapply TypeΠMatch.
+  - apply IHv. exact H7. assumption.
   - rewrite ctx_remove_extend. rewrite ctx_remove_extend.
-    assert (i+1+1=i+2) by omega. rewrite H5. apply IHc; assumption.
-+ eapply TypeΣMatch; destruct H4.
-  - apply v_negshift_typesafe. exact H9. assumption.
-  - rewrite ctx_remove_extend. apply IHc1; assumption.
-  - rewrite ctx_remove_extend. apply IHc2; assumption.
-+ eapply TypeApp; apply v_negshift_typesafe.
-  exact H5. all: assumption.
-+ eapply TypeOp. exact H8.
-  - apply v_negshift_typesafe; assumption.
+    assert (i+1+1=i+2) as SSi by omega. rewrite SSi. apply IHc; assumption.
++ specialize (v_negshift_typesafe v) as IHv.
+  specialize (c_negshift_typesafe c1) as IHc1.
+  specialize (c_negshift_typesafe c2) as IHc2.
+  clear v_negshift_typesafe c_negshift_typesafe h_negshift_typesafe.
+  simpl. inv H1. destruct no_var. destruct H0. destruct H2.
+  eapply TypeΣMatch.
+  - apply IHv. exact H9. assumption.
+  - rewrite ctx_remove_extend. apply IHc1; assumption. 
+  - rewrite ctx_remove_extend. apply IHc2; assumption. 
++ specialize (v_negshift_typesafe v) as IHv.
+  specialize (v_negshift_typesafe v0) as IHv0.
+  clear v_negshift_typesafe c_negshift_typesafe h_negshift_typesafe.
+  simpl. inv H1. destruct no_var. eapply TypeApp.
+  - apply IHv. exact H5. assumption.
+  - apply IHv0; assumption.
++ specialize (v_negshift_typesafe v) as IHv.
+  specialize (c_negshift_typesafe c) as IHc.
+  clear v_negshift_typesafe c_negshift_typesafe h_negshift_typesafe.
+  simpl. inv H1. destruct no_var. eapply TypeOp. exact H8.
+  - apply IHv; assumption.
   - rewrite ctx_remove_extend. apply IHc; assumption.
-+ eapply TypeLetRec.
++ specialize (c_negshift_typesafe c1) as IHc1.
+  specialize (c_negshift_typesafe c2) as IHc2.
+  clear v_negshift_typesafe c_negshift_typesafe h_negshift_typesafe.
+  simpl. inv H1. destruct no_var. eapply TypeLetRec.
   - rewrite ctx_remove_extend. rewrite ctx_remove_extend.
-    assert (i+1+1=i+2) by omega. rewrite H5. apply IHc1. exact H8. assumption.
-  - rewrite ctx_remove_extend. apply IHc2; assumption.
-+ eapply TypeDoBind.
+    assert (i+1+1=i+2) as SSi by omega. rewrite SSi.
+    apply IHc1. exact H8. assumption.
+  - rewrite ctx_remove_extend.  apply IHc2; assumption.
++ specialize (c_negshift_typesafe c1) as IHc1.
+  specialize (c_negshift_typesafe c2) as IHc2.
+  clear v_negshift_typesafe c_negshift_typesafe h_negshift_typesafe.
+  simpl. inv H1. destruct no_var. eapply TypeDoBind.
   - apply IHc1. exact H7. assumption.
-  - rewrite ctx_remove_extend. auto.
-+ eapply TypeHandle.
-  - apply v_negshift_typesafe. exact H5. assumption.
+  - rewrite ctx_remove_extend. apply IHc2; assumption.
++ specialize (v_negshift_typesafe v) as IHv.
+  specialize (c_negshift_typesafe c) as IHc.
+  clear v_negshift_typesafe c_negshift_typesafe h_negshift_typesafe.
+  simpl. inv H1. destruct no_var. eapply TypeHandle.
+  - apply IHv. exact H5. assumption.
   - apply IHc; assumption.
 }{
-clear h_negshift_typesafe.
-revert Γ Σ i. induction h; intros Γ Σ i orig no_var; inv orig; inv H0; inv H2;
-inv H1; apply TypeH; auto; simpl in no_var; try destruct no_var;
-try (apply ctx_remove_wf; assumption); try (apply WfCty; assumption).
-- apply WfSigØ.
-- apply TypeCasesØ.
-- apply WfSigU; assumption.
-- apply TypeCasesU.
-  assert (forall h, find_op_case h op = None 
-    -> find_op_case (Sub.h_negshift h 1 i) op = None).
-  + intro h'. induction h'; intro orig; auto.
-    simpl. simpl in orig. destruct (op==o); auto. discriminate.
-  + apply H8. assumption.
-  + auto.
-  + rewrite ctx_remove_extend. rewrite ctx_remove_extend.
-    assert (i+1+1=i+2) by omega. rewrite H8.
-    apply c_negshift_typesafe; assumption.
+intros orig no_var; simpl; apply TypeH; inv orig.
+{ apply ctx_remove_wf. assumption. }
+assumption. assumption.
+destruct h.
++ clear v_negshift_typesafe c_negshift_typesafe h_negshift_typesafe.
+  simpl. inv H2. apply TypeCasesØ.
++ specialize (h_negshift_typesafe h) as IHh.
+  specialize (c_negshift_typesafe c) as IHc.
+  clear v_negshift_typesafe c_negshift_typesafe h_negshift_typesafe.
+  simpl in no_var. destruct no_var. simpl. inv H2. apply TypeCasesU.
+  - assert (forall h,
+      find_op_case h o = None ->
+      find_op_case (Sub.h_negshift h 1 i) o = None) as no_find.
+    * intros h' orig. induction h'; auto.
+      simpl in *. destruct (o==o0). discriminate.
+      apply IHh'; assumption.
+    * apply no_find. assumption.
+  - apply IHh; assumption. 
+  - rewrite ctx_remove_extend. rewrite ctx_remove_extend.
+    assert (i+1+1=i+2) as SSi by omega. rewrite SSi. apply IHc; assumption.
 }
 Qed.
 
 
-Fixpoint v_subs_typesafe
-  (Γ:ctx) (v:val) (A:vtype) (i:nat) (v_s:val) (A_s:vtype) {struct v}:
+Fixpoint v_subs_typesafe v Γ A i v_s A_s {struct v}:
   has_vtype Γ v A -> get_vtype Γ i = Some A_s ->
   has_vtype Γ v_s A_s ->
   has_vtype Γ (Sub.v_sub v (i, v_s)) A
-with c_subs_typesafe
-  (Γ:ctx) (c:comp) (C:ctype) (i:nat) (v_s:val) (A_s:vtype) {struct c}:
+with c_subs_typesafe c Γ C i v_s A_s {struct c}:
   has_ctype Γ c C -> get_vtype Γ i = Some A_s ->
   has_vtype Γ v_s A_s ->
   has_ctype Γ (Sub.c_sub c (i, v_s)) C
-with h_subs_typesafe
-  (Γ:ctx) (h:hcases) (Σ:sig) (D:ctype) (i:nat) (v_s:val) (A_s:vtype) {struct h}:
+with h_subs_typesafe h Γ Σ D i v_s A_s {struct h}:
   has_htype Γ h Σ D -> get_vtype Γ i = Some A_s ->
   has_vtype Γ v_s A_s ->
   has_htype Γ (Sub.h_sub h (i, v_s)) Σ D.
 Proof.
+all: assert (forall i, i+1=S i) as Si by (intro; omega).
+all: assert (forall i, i+2=S(S i)) as SSi by (intro; omega).
 {
-clear v_subs_typesafe.
-revert Γ A i. induction v; intros Γ A i orig in_ctx vstyped;
-simpl; inv orig; inv H1; apply TypeV; auto.
-+ simpl in *. destruct (num=?i) eqn:cmp.
-  * apply Nat.eqb_eq in cmp. rewrite <-cmp in in_ctx.
-    rewrite H4 in in_ctx. injection in_ctx. intro samety.
-    rewrite samety. inv vstyped. assumption.
-  * apply TypeVar. assumption.
-+ apply TypeUnit.
-+ apply TypeInt.
-+ apply TypeInl. apply IHv; auto.
-+ apply TypeInr. apply IHv; auto.
-+ apply TypePair; try apply IHv1 || apply IHv2; auto.
-+ apply TypeFun. eapply c_subs_typesafe.
-  - assumption.
-  - assert (i+1=S i) by omega. rewrite H1. simpl.
-    exact in_ctx.
-  - apply v_shift_typesafe. assumption. inv H0. assumption.
-+ apply TypeHandler.
-  - eapply c_subs_typesafe.
-    * assumption.
-    * assert (i+1=S i) by omega. rewrite H1. simpl. exact in_ctx.
-    * apply v_shift_typesafe. assumption. inv H0. inv H3. assumption.
-  - eapply h_subs_typesafe.
-    * assumption.
-    * exact in_ctx.
-    * assumption.
+intros orig gets vs_types. apply TypeV; inv orig.
+assumption. assumption. destruct v.
++ clear v_subs_typesafe c_subs_typesafe h_subs_typesafe.
+  simpl. destruct v as (name, num). simpl. inv H1.
+  destruct (num =? i) eqn:cmp.
+  - apply Nat.eqb_eq in cmp. rewrite cmp in *. rewrite H6 in gets.
+    injection gets. intro. subst. inv vs_types. assumption.
+  - apply TypeVar. assumption.
++ clear v_subs_typesafe c_subs_typesafe h_subs_typesafe.
+  simpl. inv H1. apply TypeUnit.
++ clear v_subs_typesafe c_subs_typesafe h_subs_typesafe.
+  simpl. inv H1. apply TypeInt.
++ specialize (v_subs_typesafe v) as IHv.
+  clear v_subs_typesafe c_subs_typesafe h_subs_typesafe.
+  simpl. inv H1. apply TypeInl. eapply IHv.
+  assumption. exact gets. assumption.
++ specialize (v_subs_typesafe v) as IHv.
+  clear v_subs_typesafe c_subs_typesafe h_subs_typesafe.
+  simpl. inv H1. apply TypeInr. eapply IHv.
+  assumption. exact gets. assumption.
++ specialize (v_subs_typesafe v1) as IHv1.
+  specialize (v_subs_typesafe v2) as IHv2.
+  clear v_subs_typesafe c_subs_typesafe h_subs_typesafe.
+  simpl. inv H1. apply TypePair.
+  eapply IHv1. assumption. exact gets. assumption.
+  eapply IHv2. assumption. exact gets. assumption.
++ specialize (c_subs_typesafe c) as IHc.
+  specialize (v_subs_typesafe v_s) as IHvs.
+  clear v_subs_typesafe c_subs_typesafe h_subs_typesafe.
+  simpl. inv H1. apply TypeFun. eapply IHc.
+  assumption. rewrite Si. exact gets. apply v_shift_typesafe.
+  assumption. inv H0. assumption.
++ specialize (h_subs_typesafe h) as IHh.
+  specialize (c_subs_typesafe c) as IHc.
+  clear v_subs_typesafe c_subs_typesafe h_subs_typesafe.
+  simpl. inv H1. apply TypeHandler.
+  - eapply IHc. assumption. rewrite Si. exact gets.
+    apply v_shift_typesafe. assumption. inv H0. inv H3. assumption.
+  - eapply IHh. assumption. exact gets. assumption.
 }{
-clear c_subs_typesafe.
-assert (forall i, i+1=S i) as Si by (intro; omega).
-assert (forall i, i+2=S(S i)) as SSi by (intro; omega).
-revert Γ C i v_s. induction c; intros Γ C i v_s orig in_ctx vstyped;
-simpl; inv orig; inv H1; apply TypeC; auto.
-+ apply TypeRet. eapply v_subs_typesafe. 2 : exact in_ctx. all: assumption.
-+ eapply TypeΠMatch.
-  - eapply v_subs_typesafe. exact H7. exact in_ctx. assumption.
-  - apply IHc. assumption.
-    * rewrite SSi. assumption.
-    * rewrite <-(v_shift_shift 1 1 0).
-      apply v_shift_typesafe. apply v_shift_typesafe. assumption.
-      all: (inv H7; inv H2; assumption).
-+ eapply TypeΣMatch.
-  { eapply v_subs_typesafe. exact H9. exact in_ctx. assumption. }
-  all: try apply IHc1 || apply IHc2; try apply v_shift_typesafe; auto.
-  all: try (rewrite Si; assumption).
-  all: inv H9; inv H2; assumption.
-+ eapply TypeApp.
-  - eapply v_subs_typesafe. exact H5. exact in_ctx. assumption.
-  - eapply v_subs_typesafe. auto. exact in_ctx. assumption.
-+ eapply TypeOp. exact H8.
-  - eapply v_subs_typesafe. 2: exact in_ctx. assumption. assumption.
-  - apply IHc; auto.
-    * rewrite Si. assumption.
-    * apply v_shift_typesafe. assumption. inv H0.
-      eapply get_op_type_wf. exact H5. exact H8.
-+ eapply TypeLetRec.
-  - apply IHc1. exact H8.
-    * rewrite SSi. assumption.
-    * rewrite <-(v_shift_shift 1 1 0).
-      apply v_shift_typesafe. apply v_shift_typesafe. assumption.
-      ++ inv H9. inv H1. inv H7. assumption.
-      ++ inv H9. inv H1. assumption.
-  - apply IHc2. assumption.
-    * rewrite Si. assumption.
-    * apply v_shift_typesafe. assumption.
-      inv H9. inv H1. assumption.
-+ eapply TypeDoBind.
-  - apply IHc1. exact H7. assumption. assumption.
-  - apply IHc2.
-    * assumption.
-    * rewrite Si. assumption.
-    * apply v_shift_typesafe. assumption. inv H7. inv H2. assumption.
-+ eapply TypeHandle.
-  - eapply v_subs_typesafe. exact H5. exact in_ctx. assumption.
-  - apply IHc; auto.
+intros orig gets vs_types. apply TypeC; inv orig.
+assumption. assumption. destruct c.
++ specialize (v_subs_typesafe v) as IHv.
+  clear v_subs_typesafe c_subs_typesafe h_subs_typesafe.
+  simpl. inv H1. apply TypeRet. eapply IHv.
+  assumption. exact gets. assumption.
++ specialize (v_subs_typesafe v) as IHv.
+  specialize (c_subs_typesafe c) as IHc.
+  clear v_subs_typesafe c_subs_typesafe h_subs_typesafe.
+  simpl. inv H1. eapply TypeΠMatch.
+  - eapply IHv. exact H7. exact gets. assumption.
+  - eapply IHc. assumption. rewrite SSi. exact gets. 
+    rewrite <-(v_shift_shift 1 1 0).
+    apply v_shift_typesafe. apply v_shift_typesafe. assumption.
+    all: inv H7; inv H2; assumption.
++ specialize (v_subs_typesafe v) as IHv.
+  specialize (c_subs_typesafe c1) as IHc1.
+  specialize (c_subs_typesafe c2) as IHc2.
+  clear v_subs_typesafe c_subs_typesafe h_subs_typesafe.
+  simpl. inv H1. eapply TypeΣMatch.
+  - eapply IHv. exact H9. exact gets. assumption.
+  - eapply IHc1. assumption. rewrite Si. exact gets.
+    apply v_shift_typesafe. assumption.
+    inv H9. inv H2. assumption. 
+  - eapply IHc2. assumption. rewrite Si. exact gets.
+    apply v_shift_typesafe. assumption.
+    inv H9. inv H2. assumption. 
++ specialize (v_subs_typesafe v) as IHv.
+  specialize (v_subs_typesafe v0) as IHv0.
+  clear v_subs_typesafe c_subs_typesafe h_subs_typesafe.
+  simpl. inv H1. eapply TypeApp.
+  - eapply IHv. exact H5. exact gets. assumption.
+  - eapply IHv0. assumption. exact gets. assumption.
++ specialize (v_subs_typesafe v) as IHv.
+  specialize (c_subs_typesafe c) as IHc.
+  clear v_subs_typesafe c_subs_typesafe h_subs_typesafe.
+  simpl. inv H1. eapply TypeOp. exact H8.
+  - eapply IHv. assumption. exact gets. assumption.
+  - eapply IHc. assumption. rewrite Si. exact gets. 
+    apply v_shift_typesafe. assumption.
+    inv H10. inv H1. assumption.
++ specialize (c_subs_typesafe c1) as IHc1.
+  specialize (c_subs_typesafe c2) as IHc2.
+  clear v_subs_typesafe c_subs_typesafe h_subs_typesafe.
+  simpl. inv H1. eapply TypeLetRec.
+  - rewrite SSi. eapply IHc1. exact H8. exact gets.
+    rewrite <-(v_shift_shift 1 1 0).
+    apply v_shift_typesafe. apply v_shift_typesafe. assumption.
+    all: inv H8; inv H1. 2: assumption. inv H6. assumption. 
+  - eapply IHc2. assumption. rewrite Si. exact gets.
+    apply v_shift_typesafe. assumption.
+    inv H9. inv H1. assumption.
++ specialize (c_subs_typesafe c1) as IHc1.
+  specialize (c_subs_typesafe c2) as IHc2.
+  clear v_subs_typesafe c_subs_typesafe h_subs_typesafe.
+  simpl. inv H1. eapply TypeDoBind.
+  - eapply IHc1. exact H7. exact gets. assumption.
+  - eapply IHc2. assumption. rewrite Si. exact gets.
+    apply v_shift_typesafe. assumption.
+    inv H7. inv H2. assumption.
++ specialize (v_subs_typesafe v) as IHv.
+  specialize (c_subs_typesafe c) as IHc.
+  clear v_subs_typesafe c_subs_typesafe h_subs_typesafe.
+  simpl. inv H1. eapply TypeHandle.
+  - eapply IHv. exact H5. exact gets. assumption.
+  - eapply IHc. assumption. exact gets. assumption.
 }{
-clear h_subs_typesafe.
-assert (forall i, i+1=S i) as Si by (intro; omega).
-assert (forall i, i+2=S(S i)) as SSi by (intro; omega).
-revert Γ Σ D i v_s. induction h; intros Γ Σ D i v_s orig in_ctx vstyped;
-simpl; inv orig; inv H2; apply TypeH; auto.
-+ apply TypeCasesØ.
-+ apply TypeCasesU.
-  assert (forall h,
-    find_op_case h o = None ->
-    find_op_case (Sub.h_sub h (i, v_s)) o = None).
-  * intros h' cantfind. induction h'. auto.
-    simpl. simpl in cantfind. destruct (o==o0). discriminate.
-    apply IHh'. exact cantfind.
-  * apply H2. assumption.
-  * auto.
-  * rewrite SSi. eapply c_subs_typesafe; auto.
-    - simpl. exact in_ctx.
-    - rewrite <-(v_shift_shift 1 1 0).
-      apply v_shift_typesafe. apply v_shift_typesafe. assumption.
+intros orig gets vs_types; simpl; apply TypeH; inv orig.
+assumption. assumption. assumption.
+destruct h.
++ clear v_subs_typesafe c_subs_typesafe h_subs_typesafe.
+  inv H2. apply TypeCasesØ.
++ specialize (h_subs_typesafe h) as IHh.
+  specialize (c_subs_typesafe c) as IHc.
+  clear v_subs_typesafe c_subs_typesafe h_subs_typesafe.
+  simpl. inv H2. apply TypeCasesU.
+  - assert (forall h,
+      find_op_case h o = None ->
+      find_op_case (Sub.h_sub h (i, v_s)) o = None) as no_find.
+    * intros h' orig. induction h'; auto.
+      simpl in *. destruct (o==o0). discriminate.
+      apply IHh'. assumption.
+    * apply no_find. assumption.
+  - eapply IHh. exact H12. exact gets. assumption.
+  - rewrite SSi. eapply IHc. assumption. exact gets.
+    rewrite <-(v_shift_shift 1 1 0).
+    apply v_shift_typesafe. apply v_shift_typesafe. assumption.
+    all: inv H0. 2: assumption. inv H12. apply WfFun; assumption.
 }
 Qed.
+
 
 Lemma h_has_case Γ h Σ D op A_op B_op:
   has_htype Γ h Σ D ->
@@ -744,4 +468,3 @@ inv typed; inv H1; inv H2.
     exists v. exists v0. exists c. reflexivity.
   - apply IHh in H14; assumption.
 Qed.
-*)
