language_formalisation/type_system/type_lemmas.v
@@ -6,7 +6,7 @@ Add LoadPath "C:\Users\Ziga\Documents\Ziga_podatki\PHD\language_formalisation\op
 (* Add LoadPath "E:\Ziga_Podatki\faks\PHD\language_formalisation\substitution". *)
 (* Add LoadPath "E:\Ziga_Podatki\faks\PHD\language_formalisation\type_system". *)
 (* Add LoadPath "E:\Ziga_Podatki\faks\PHD\language_formalisation\operational_semantics". *)
-Require Export syntax bidirectional substitution
+Require Export syntax declarational substitution
   subs_lemmas Omega Logic type_aux_lemmas operational_semantics.
 
 
@@ -30,21 +30,21 @@ intros orig sub. unfold v_sub_out.
 assert (Γ = ctx_remove_var (CtxU Γ A_s) 0) by auto.
 rewrite H. apply v_negshift_typesafe.
 eapply v_subs_typesafe. assumption. simpl. reflexivity.
-apply v_shift_typesafe. assumption.
+apply v_shift_typesafe. assumption. inv sub. assumption.
 apply v_no_var_sub. apply v_shift_makes_no_var.
 }{
 intros orig sub. unfold c_sub_out.
 assert (Γ = ctx_remove_var (CtxU Γ A_s) 0) by auto.
 rewrite H. apply c_negshift_typesafe.
 eapply c_subs_typesafe. assumption. simpl. reflexivity.
-apply v_shift_typesafe. assumption.
+apply v_shift_typesafe. assumption. inv sub. assumption.
 apply c_no_var_sub. apply v_shift_makes_no_var.
 }{
 intros orig sub. unfold h_sub_out.
 assert (Γ = ctx_remove_var (CtxU Γ A_s) 0) by auto.
 rewrite H. apply h_negshift_typesafe.
 eapply h_subs_typesafe. assumption. simpl. reflexivity.
-apply v_shift_typesafe. assumption.
+apply v_shift_typesafe. assumption. inv sub. assumption.
 apply h_no_var_sub. apply v_shift_makes_no_var.
 }
 Qed.
@@ -52,59 +52,77 @@ Qed.
 Lemma preservation Γ c c' C:
   has_ctype Γ c C -> step c c' -> has_ctype Γ c' C.
 Proof.
-intros orig step. revert C orig. induction step; intros C orig; inv orig.
-+ inv H5.
+intros orig step. revert C orig. 
+induction step; intros C orig; inv orig; inv H1.
++ inv H8. inv H3.
   unfold c_sub2_out.
-  eapply c_sub_out_typesafe. 2: exact H3.
-  eapply c_sub_out_typesafe. exact H6.
-  apply v_shift_typesafe. assumption.
-+ inv H6.
-  eapply c_sub_out_typesafe. exact H7. assumption.
-+ inv H6.
-  eapply c_sub_out_typesafe. exact H8. assumption.
-+ inv H2.
-  eapply c_sub_out_typesafe. exact H1. assumption.
-+ eapply c_sub_out_typesafe. exact H6.
-  apply TypeFun. eapply TypeLetRec. 2: exact H5.
-  assert (CtxU (CtxU (CtxU Γ A) A) (TyFun A C0) 
-    = ctx_insert_var (CtxU (CtxU Γ A) (TyFun A C0)) A 2).
-  simpl. destruct Γ; auto.
-  rewrite H.
-  apply c_insert_typesafe. assumption.
-+ eapply TypeDoBind. 2: exact H5. auto.
-+ eapply c_sub_out_typesafe. exact H5. inv H4. assumption.
-+ inv H4. eapply TypeOp. exact H3. assumption.
-  eapply TypeDoBind. exact H11. 
-  assert (CtxU (CtxU Γ B_op) A 
-    = ctx_insert_var (CtxU Γ A) B_op 1).
-  simpl. destruct Γ; auto.
-  rewrite H. apply c_insert_typesafe. assumption.
-+ eapply TypeHandle. exact H2. apply IHstep. assumption.
-+ inv H2. eapply c_sub_out_typesafe. exact H3. inv H4. assumption.
-+ unfold c_sub2_out. inv H5.
+  eapply c_sub_out_typesafe. 2: exact H8.
+  eapply c_sub_out_typesafe. exact H9.
+  apply v_shift_typesafe. assumption. inv H8. assumption.
++ inv H9. inv H3.
+  eapply c_sub_out_typesafe. exact H10. assumption.
++ inv H9. inv H3.
+  eapply c_sub_out_typesafe. exact H11. assumption.
++ inv H5. inv H3.
+  eapply c_sub_out_typesafe. exact H6. assumption.
++ eapply c_sub_out_typesafe. exact H9.
+  apply TypeV. assumption. inv H9. inv H1. assumption. 
+  apply TypeFun. apply TypeC.
+  - inv H8. inv H1. assumption.
+  - inv H8. assumption.
+  - eapply TypeLetRec. 2: exact H8.
+    assert (CtxU (CtxU (CtxU Γ A) A) (TyFun A C0) 
+      = ctx_insert_var (CtxU (CtxU Γ A) (TyFun A C0)) A 2)
+    as insertion.
+    { simpl. destruct Γ; auto. }
+    rewrite insertion.
+    apply c_insert_typesafe. assumption.
+    inv H8. inv H1. inv H6. assumption.
++ apply TypeC. assumption. assumption.
+  eapply TypeDoBind. 2: exact H8. auto.
++ eapply c_sub_out_typesafe. exact H8. inv H7. inv H3. assumption.
++ inv H7. inv H3. apply TypeC. assumption. assumption.
+  eapply TypeOp. exact H9. assumption.
+  apply TypeC. inv H15. assumption. assumption.
+  eapply TypeDoBind. exact H15. 
+  assert (CtxU (CtxU Γ B_op) A = ctx_insert_var (CtxU Γ A) B_op 1).
+  { simpl. destruct Γ; auto. }
+  rewrite H3. apply c_insert_typesafe. assumption.
+  inv H15. inv H4. assumption.
++ apply TypeC. assumption. assumption.
+  eapply TypeHandle. exact H5. apply IHstep. assumption.
++ inv H5. inv H3. eapply c_sub_out_typesafe. 
+  - exact H8.
+  - inv H7. inv H5. assumption.
++ unfold c_sub2_out. inv H2. inv H10. inv H6.
   eapply c_sub_out_typesafe.
-  Focus 2.
-    apply TypeFun. eapply TypeHandle.
-    apply v_shift_typesafe. exact H3. exact H10.
-  inv H3.
-  assert (forall h Σ,
-    find_op_case h op_id = Some (x_op, k_op, c_op) ->
-    get_op_type Σ op_id = Some (A_op, B_op) ->
-    has_htype Γ h Σ C ->
-    has_ctype (CtxU Γ (TyFun B_op C))
-      (c_sub_out c_op (Sub.v_shift v_arg 1 0)) C).
-  - intro h'. induction h'; intros Σ' finds gets types.
-    * simpl in finds. discriminate.
-    * clear H8 H4 H13.
-      simpl in finds. inv types; destruct (op_id==o) eqn:name; simpl.
-      ++ injection finds. intros. subst.
-         simpl in gets. rewrite name in gets.
-         injection gets. intros. subst.
-         eapply c_sub_out_typesafe. exact H12.
-         apply v_shift_typesafe. assumption.
-      ++ eapply IHh'; simpl in gets; rewrite name in gets.
-         assumption. exact gets. assumption. 
-  - eapply H0. exact H. exact H8. assumption. 
+  instantiate (1 := TyFun B_op (CTy A Σ E)).
+  - assert (forall h C Σ,
+      find_op_case h op_id = Some (x_op, k_op, c_op) ->
+      get_op_type Σ op_id = Some (A_op, B_op) ->
+      has_htype Γ h Σ C ->
+      has_ctype (CtxU Γ (TyFun B_op C))
+        (c_sub_out c_op (Sub.v_shift v_arg 1 0)) C).
+    -- intros h' C. induction h'; intros Σ' finds gets types.
+      * simpl in finds. discriminate.
+      * simpl in finds. inv types. inv H10. simpl in gets.
+        destruct (op_id==o).
+        ++ injection finds. injection gets. intros. subst. 
+          eapply c_sub_out_typesafe. exact H24.
+          apply v_shift_typesafe. assumption.
+          inv H24. inv H10. inv H18. assumption.
+        ++ eapply IHh'. assumption. exact gets. assumption.
+    -- eapply H6. exact H. exact H14. inv H8. inv H10. assumption.
+  - apply TypeV. assumption. 
+    * apply WfFun. inv H16. inv H6. assumption. apply WfCty; assumption.
+    * apply TypeFun. apply TypeC.
+      { inv H16. assumption. }
+      { apply WfCty; assumption. }
+      inv H8. eapply TypeHandle.
+      apply v_shift_typesafe.
+      { apply TypeV. assumption. exact H7. assumption. }
+      { inv H16. inv H8. assumption. }
+      assumption.
 Qed.
 
 Lemma progress c C:
@@ -114,46 +132,35 @@ Lemma progress c C:
 Proof.
 revert C. induction c; intros C orig.
 + left. exists v. reflexivity.
-+ right. right. inv orig. destruct v; inv H4.
++ right. right. inv orig. inv H1. inv H7. inv H3.
   - simpl in H1. discriminate.
   - eexists. apply Step_ΠMatch.
 + right. right. rename v0 into x. rename v1 into y.
-  inv orig. destruct v; inv H6.
+  inv orig. inv H1. inv H9; inv H3.
   - simpl in H1. discriminate.
   - eexists. apply Step_ΣMatch_Inl.
   - eexists. apply Step_ΣMatch_Inr.
-+ right. right. inv orig. destruct v; inv H2.
++ right. right. inv orig. inv H1. inv H5; inv H3.
   - simpl in H1. discriminate.
   - eexists. apply Step_App.
 + right. left. exists o. exists v. exists v0. exists c. reflexivity.
 + right. right. rename v into f. rename v0 into x.
   eexists. apply Step_LetRec.
-+ right. right. rename v into x. inv orig.
-  apply IHc1 in H4. destruct H4 as [h1 | [h2 | h3]].
-  - destruct h1. rewrite H in *. eexists. apply Step_DoBind_Ret.
-  - destruct h2. destruct H. destruct H. destruct H. rewrite H in *.
++ right. right. rename v into x. inv orig. inv H1.
+  apply IHc1 in H7. destruct H7 as [h1 | [h2 | h3]].
+  - destruct h1. rewrite H1 in *. eexists. apply Step_DoBind_Ret.
+  - destruct h2. destruct H1. destruct H1. destruct H1. rewrite H1 in *.
     eexists. apply Step_DoBind_Op.
-  - destruct h3. eexists. apply Step_DoBind_step. exact H.
-+ right. right. inv orig. inv H2. { simpl in H. discriminate. }
-  apply IHc in H4 as IH. destruct IH as [h1 | [h2 | h3]].
-  - destruct h1. rewrite H in *. eexists. apply Step_Handle_Ret.
-  - destruct h2. destruct H. destruct H. destruct H. rewrite H in *.
+  - destruct h3. eexists. apply Step_DoBind_step. exact H1.
++ right. right. inv orig. inv H1. inv H5. inv H3. { simpl in H4. discriminate. }
+  apply IHc in H7 as IH. destruct IH as [h1 | [h2 | h3]].
+  - destruct h1. rewrite H3 in *. eexists. apply Step_Handle_Ret.
+  - destruct h2. destruct H3. destruct H3. destruct H3. rewrite H3 in *.
     rename x0 into o. rename x1 into v_arg. rename x2 into y. rename x3 into k. 
-    inv H4. specialize (h_has_case CtxØ h sig C o A_op B_op H6 H7) as gets.
-    destruct gets. destruct H. destruct H.
-    eexists. eapply Step_Handle_Op. exact H.
+    inv H7. inv H6. 
+    specialize (h_has_case CtxØ h Σ C o A_op B_op H10 H12) as gets.
+    destruct gets. destruct H3. destruct H3.
+    eexists. eapply Step_Handle_Op. exact H3.
   - destruct h3 as [c' h3].
     eexists. eapply Step_Handle_Step. exact h3.
 Qed.
-
-
-
-
-
-
-
-
-
-
-
-
